src/Interfaces.v
@@ -5,12 +5,12 @@ From Equations Require Import Equations.
 
 From Coq Require Import Arith List Lia Setoid Morphisms.
 Import ListNotations.
-From Clairvoyance Require Import Core Approx ApproxM List Misc BankersQueue Cost.
+From Clairvoyance Require Import Core Approx ApproxM List Misc Cost.
 
 Set Primitive Projections.
-Set Implicit Arguments.
+(* Set Implicit Arguments.
 Set Contextual Implicit.
-Set Maximal Implicit Insertion.
+Set Maximal Implicit Insertion. *)
 
 (* lookups xs [n; m; p] = [xs!!n; xs!!m; xs!!p], or None if out of bounds *)
 Fixpoint lookups {A} (xs : list A) (ns : list nat) : option (list A) :=
@@ -26,11 +26,11 @@ Class PureImpl (op value : Type) : Type :=
 
 Definition event (op : Type) : Type := (op * list nat).
 Definition trace (op : Type) : Type := list (event op).
-Definition stack (value : Type) : Type := list value.
+Notation stack := list (only parsing).
 
 Section Pure.
 
-Context {op value : Type} {j : PureImpl op value}.
+Context {op value : Type} {pure_impl : PureImpl op value}.
 
 Definition eval_event '((o, ns) : event op) (vs : stack value) : stack value :=
   match lookups vs ns with
@@ -38,11 +38,13 @@ Definition eval_event '((o, ns) : event op) (vs : stack value) : stack value :=
   | Some xs => vs ++ eval_op o xs
   end.
 
-Fixpoint eval_trace (es : trace op) (xs : stack value) : stack value :=
+Fixpoint eval_trace_from (es : trace op) (xs : stack value) : stack value :=
   match es with
   | [] => xs
-  | e :: es => eval_trace es (eval_event e xs)
+  | e :: es => eval_trace_from es (eval_event e xs)
   end.
+
+Definition eval_trace (es : trace op) : stack value := eval_trace_from es [].
 
 End Pure.
 
@@ -60,11 +62,13 @@ Definition cost_event '((o, ns) : event op) (vs : stack value) : nat :=
   | Some xs => cost_op o xs
   end.
 
-Fixpoint cost_trace (es : trace op) (vs : stack value) : nat :=
+Fixpoint cost_trace_from (es : trace op) (vs : stack value) : nat :=
   match es with
   | [] => 0
-  | e :: es => cost_event e vs + cost_trace es (eval_event e vs)
+  | e :: es => cost_event e vs + cost_trace_from es (eval_event e vs)
   end.
+
+Definition cost_trace (es : trace op) : nat := cost_trace_from es [].
 
 End Cost.
 
@@ -78,62 +82,150 @@ Context {op valueA : Type} {cv_impl : CvImpl op valueA}.
 Definition exec_event '((o, ns) : event op) (vs : stack valueA) : M (stack valueA) :=
   match lookups vs ns with
   | None => ret vs  (* noop *)
-  | Some xs => let! ys := exec_op o xs in ret (xs ++ vs)
+  | Some xs => let! ys := exec_op o xs in ret (vs ++ ys)
   end.
 
-Fixpoint exec_trace (es : trace op) (vs : stack valueA) : M (stack valueA) :=
+Fixpoint exec_trace_from (es : trace op) (vs : stack valueA) : M (stack valueA) :=
   match es with
   | [] => ret vs
-  | e :: es => let! vs := exec_event e vs in exec_trace es vs
+  | e :: es => let! vs := exec_event e vs in exec_trace_from es vs
   end.
+
+Definition exec_trace (es : trace op) : M (stack valueA) :=
+  exec_trace_from es [].
 
 End Cv.
 
-Section Obligations.
-
-Context (op value valueA : Type) {pure_impl : PureImpl op value} {cv_impl : CvImpl op valueA}.
-
-(** Order structure on approximation values [valueA]. *)
-Class ImplApprox : Type :=
-  { ImplExact :> Exact value valueA
-  ; ImplLessDefined :> LessDefined valueA
-  ; ImplPreOrder :> PreOrder (less_defined (a := valueA))
-  ; ImplLub :> Lub valueA
-  ; ImplLubLaw :> LubLaw valueA
-  ; exec_op_mon :> forall o,
-      Proper (less_defined ==> less_defined) (exec_op (valueA := valueA) o)
+(** Order structure on approximation values [valueA].
+    Core operations ([exact], [less_defined], [lub], [bottom_of])
+    and their properties. *)
+Class ApproxOrder (op value valueA : Type) : Type :=
+  { AO_Exact :> Exact value valueA
+  ; AO_LessDefined :> LessDefined valueA
+  ; AO_PreOrder :> PreOrder (less_defined (a := valueA))
+  ; AO_Lub :> Lub valueA
+  ; AO_LubLaw :> LubLaw valueA
+  ; AO_HasBottom :> HasBottom valueA
+  ; AO_BottomIsLeast :> BottomIsLeast valueA
   }.
+
+(* Monotonicity of [exec_op] *)
+Class MonotoneCvImpl {op value valueA}
+    {approx_order : ApproxOrder op value valueA}
+    (cv_impl : CvImpl op valueA) : Prop :=
+  exec_op_mon : forall o, Proper (less_defined ==> less_defined) (exec_op (valueA := valueA) o).
+
+(** Amortized cost specification. *)
+Section HasAmortizedCost.
+
+Context {op value valueA : Type}
+  {pure_impl : PureImpl op value}
+  {cost_spec : CostSpec op value}
+  {cv_impl : CvImpl op valueA}.
+
+(** The cost of executing the whole trace is less than
+    its aggregated bound. *)
+Definition HasAmortizedCost : Prop :=
+  forall os : trace op,
+    (cost_of (exec_trace os) <= cost_trace os)%NAT.
+
+(** Equivalent formulation as a weakest precondition. *)
+Definition HasAmortizedCost' : Prop :=
+  forall os : trace op,
+    exec_trace os [[ fun _ c => c <= cost_trace os ]].
+
+Context
+  {approx_order : ApproxOrder op value valueA}.
+
+Theorem has_amortized_cost' :
+  HasAmortizedCost <-> HasAmortizedCost'.
+Admitted.
+
+End HasAmortizedCost.
+
+Arguments HasAmortizedCost : clear implicits.
+Arguments HasAmortizedCost {op value valueA pure_impl} cost_spec cv_impl.
+
+Arguments HasAmortizedCost' : clear implicits.
+Arguments HasAmortizedCost' {op value valueA pure_impl} cost_spec cv_impl.
+
+(** Clairvoyant Physicist's method *)
+
+(* TODO: These classes are a bit of a mess. Find a good way to package all of the required operations and facts together. *)
+
+Class Potential (a : Type) : Type :=
+  potential : a -> nat.
 
 Definition sumof {A} (f : A -> nat) : list A -> nat :=
   fold_right (fun x s => f x + s) 0.
 
-Context {cost_spec : CostSpec op value}.
+#[global]
+Instance Potential_list {a} `{Potential a} : Potential (list a) := sumof potential.
 
-(** Theorem statement: "the implementation [cv_impl] simulates [pure_impl]
-    with amortized cost bounded above by [cost_spec]." *)
-Class HasAmortizedCost {IA : ImplApprox} : Type :=
-  { potential : valueA -> nat
-  ; potentials := sumof potential
-  ; potential_lub : forall x y, cobounded x y -> potential (lub x y) <= potential x + potential y
+Class PotentialLub (a : Type) `{Potential a, LessDefined a, Lub a} : Prop :=
+  potential_lub : forall x y : a, cobounded x y -> potential (lub x y) <= potential x + potential y.
 
-    (* Note: lazy evaluation works backwards. We are first given an [output] demand,
-       obtained as an approximation of the reference output via [eval_op],
-       and we have to find a matching [input] demand. *)
-  ; exec_cost : forall (o : op) (vs : list value),
-      forall output, output `is_approx` eval_op o vs ->
-      exists input, input `is_approx` vs /\
-      exec_op o input [[ fun r c =>
-        output `less_defined` r /\
-        potentials input + c <= cost_op o vs + potentials output ]]
+#[global]
+Instance PotentialLub_list {a} `{PotentialLub a} : PotentialLub (list a).
+Proof.
+  intros x y.
+  induction 1 as [ | ? ? ? ? ? ? IH ] using cobounded_list_ind;
+    cbn; [ reflexivity | ].
+  rewrite IH, potential_lub by assumption.
+  clear. generalize (potential x) (potential y). lia.
+Qed.
+
+Lemma potential_app {a} `{Potential a} (x y : list a)
+  : potential (x ++ y) = potential x + potential y.
+Proof.
+  induction x as [ | x0 ? IH ]; cbn; [ auto | rewrite IH ]. lia.
+Qed.
+
+Class PotentialBottom (a : Type) `{Potential a, HasBottom a} : Prop :=
+  potential_bottom : forall x : a, potential (bottom_of x) = 0.
+
+#[global] Instance PotentialBottom_list {a} `{PotentialBottom a} : PotentialBottom (list a).
+Proof.
+  intros x; induction x as [ | ? ? IH ]; cbn; [ reflexivity | ].
+  rewrite potential_bottom, IH. reflexivity.
+Qed.
+
+Class HasPotential {op value} valueA
+    {approx_order : ApproxOrder op value valueA} : Type :=
+  { _Potential :> Potential valueA
+  ; _PotentialLub :> PotentialLub valueA
+  ; _PotentialBottom :> PotentialBottom valueA
   }.
 
-End Obligations.
+Section Physicist'sArgument.
 
-Arguments ImplApprox : clear implicits.
-Arguments ImplApprox op value valueA {_}.
+Context {op value valueA : Type}
+  {approx_order : ApproxOrder op value valueA}
+  {pure_impl : PureImpl op value}
+  {cost_spec : CostSpec op value}
+  {cv_impl : CvImpl op valueA}.
 
-Arguments HasAmortizedCost : clear implicits.
-Arguments HasAmortizedCost op value valueA {_ _ _ _}.
+(** Theorem statement: "the implementation [cv_impl] simulates [pure_impl]
+    with amortized cost bounded above by [cost_spec] plus a potential
+    difference." *)
+(* Note: lazy evaluation works backwards.
+   We are first given an [output] demand,
+   obtained as an approximation of the reference output via [eval_op],
+   and we have to find a matching [input] demand. *)
+Class Physicist'sArgument : Type :=
+  { for_some_potential :> HasPotential valueA
+  ; exec_cost : forall (o : op) (vs : list value),
+      forall output : stack valueA, output `is_approx` eval_op o vs ->
+      exists input : stack valueA, input `is_approx` vs /\
+      exec_op o input [[ fun r c =>
+        output `less_defined` r /\
+        potential input + c <= cost_op o vs + potential output ]]
+  }.
+
+End Physicist'sArgument.
+
+Arguments Physicist'sArgument : clear implicits.
+Arguments Physicist'sArgument {op value valueA approx_order pure_impl} cost_spec cv_impl.
 
 (* Auxiliary lemmas *)
 
@@ -187,29 +279,19 @@ Qed.
 Section Soundness.
 
 Context {op value valueA : Type}
-  {pure_impl : PureImpl op value} {cost_spec : CostSpec op value} {cv_impl : CvImpl op valueA}
-  {IA : ImplApprox op value valueA} {IC : HasAmortizedCost op value valueA}.
-
-Lemma potentials_lub x y : cobounded x y -> potentials (lub x y) <= potentials x + potentials y.
-Proof.
-  induction 1 as [ | ? ? ? ? ? ? IH ] using cobounded_list_ind;
-    cbn; [ reflexivity | ].
-  rewrite IH, potential_lub by assumption.
-  clear. generalize (potential x) (potential y). lia.
-Qed.
-
-Lemma potentials_app x y : potentials (x ++ y) = potentials x + potentials y.
-Proof.
-  induction x as [ | ? ? IH ]; cbn; [ auto | rewrite IH ].
-  generalize (potential a); lia.
-Qed.
+  {approx_order : ApproxOrder op value valueA}
+  {pure_impl : PureImpl op value}
+  {cost_spec : CostSpec op value}
+  {cv_impl : CvImpl op valueA}
+  {monotone_cv_impl : MonotoneCvImpl cv_impl}
+  {pa : Physicist'sArgument cost_spec cv_impl}.
 
 Lemma exec_cost_event (e : event op) (vs : stack value) output
   : output `is_approx` eval_event e vs ->
     exists input, input `is_approx` vs /\
     exec_event e input [[ fun r c =>
       output `less_defined` r /\
-      potentials input + c <= cost_event e vs + potentials output ]].
+      potential input + c <= cost_event e vs + potential output ]].
 Proof.
   destruct e as [o ns].
   unfold eval_event, exec_event.
@@ -217,29 +299,28 @@ Proof.
   - rewrite exact_list_app in Hout. apply less_defined_app_inv in Hout.
     destruct Hout as (out1 & out2 & Hout & Hout1 & Hout2).
     apply exec_cost in Hout2. destruct Hout2 as (input & Hin & HH).
-    destruct (less_defined_lookups (f := potential) E Hin) as (input' & Hin' & Hpotential & HH').
+    destruct (less_defined_lookups (f := potential) E _ Hin) as (input' & Hin' & Hpotential & HH'); change (sumof (A := valueA) potential) with (potential (a := list valueA)) in Hpotential.
     exists (lub input' out1).
     split; [ apply lub_least_upper_bound; auto | ].
     destruct (lookups_lub (ys := out1) HH') as (y1 & Hx & Hcob1 & Hy);
       [ eauto | ].
     rewrite Hy.
-    mgo. relax; [ | intros ? ? Hr; mgo; rewrite Nat.add_0_r; exact Hr ].
+    mgo_. relax; [ | intros ? ? Hr; mgo_; rewrite Nat.add_0_r; exact Hr ].
     eapply optimistic_corelax;
       [ eapply exec_op_mon, lub_upper_bound_l; eauto | | ].
     { unfold uc; intros * ? ? []; split.
-      - rewrite H1. apply less_defined_app; try reflexivity.
+      - rewrite H1. apply less_defined_app; reflexivity + assumption.
       - rewrite <- H2. lia. }
     relax; [ apply HH | cbn; intros r c [Hr Hc] ].
-    split; [ rewrite Hout; apply less_defined_app | ].
-    { admit. } { admit. }
-    rewrite potentials_lub by eauto. rewrite Hout, potentials_app.
-    unfold potentials, cost_event. rewrite E, Hpotential.
+    split; [ rewrite Hout; apply less_defined_app; [ apply lub_upper_bound_r; eauto | assumption ] | ].
+    rewrite potential_lub by eauto. rewrite Hout, potential_app.
+    rewrite E, Hpotential.
     revert Hc. generalize (cost_op o l). lia.
   - exists output. rewrite (less_defined_lookups_None E Hout).
-    split; [ auto | ]. mgo. split; [ reflexivity | lia ].
-Admitted.
+    split; [ auto | ]. mgo_. split; [ reflexivity | lia ].
+Qed.
 
-Lemma eval_trace_mon os : Proper (less_defined ==> less_defined) (exec_trace os).
+Lemma eval_trace_from_mon os : Proper (less_defined ==> less_defined) (exec_trace_from os).
 Proof.
 Admitted.
 
@@ -252,37 +333,38 @@ Proof.
   rewrite <- Hf. apply Hg.
 Qed.
 
-Lemma HasAmortizedCostSoundnessSoundness_aux
+Lemma physicist's_argument_soundness_aux
   : forall (os : trace op) (vs : list value),
-    forall output, output `is_approx` eval_trace os vs ->
+    forall output, output `is_approx` eval_trace_from os vs ->
     exists input, input `is_approx` vs /\
-      exec_trace os input [[ fun r c =>
-        output `less_defined` r /\ potentials input + c <= cost_trace os vs + potentials output ]].
+      exec_trace_from os input [[ fun r c =>
+        output `less_defined` r /\ potential input + c <= cost_trace_from os vs + potential output ]].
 Proof.
   induction os as [ | [o ns] os IH ]; intros vs output Hout; cbn.
   - exists output. split; [apply Hout | ].
     apply optimistic_ret. split; [ reflexivity | lia ].
   - cbn in Hout. specialize (IH (eval_event (o, ns) vs) output Hout).
     destruct IH as (input & Hin & IH).
-    destruct (exec_cost_event _ _ Hin) as (inp & Hinp & HH).
+    destruct (exec_cost_event _ _ _ Hin) as (inp & Hinp & HH).
     exists inp. split; [ auto | ].
-    mgo. relax; [ apply HH | cbn; intros ? ? [HI HJ] ].
-    eapply optimistic_corelax; [ apply eval_trace_mon; eassumption | | ].
+    mgo_. relax; [ apply HH | cbn; intros ? ? [HI HJ] ].
+    eapply optimistic_corelax; [ apply eval_trace_from_mon; eassumption | | ].
     { eapply uc_ext; [ intros ? ?; rewrite Nat.add_assoc; reflexivity | apply uc_acost ]. }
     relax; [ apply IH | cbn; intros ? ? [HK HL] ].
     split; [ auto | ].
     lia.
 Qed.
 
-Theorem HasAmortizedCostSoundnessSoundness
-  : forall os : trace op,
-    forall d, d `is_approx` eval_trace os [] ->
-      exec_trace os [] [[ fun r c =>
-        d `less_defined` r /\ c <= cost_trace os [] + potentials d ]].
+Theorem physicist's_argument_soundness : HasAmortizedCost cost_spec cv_impl.
 Proof.
-  intros os d Hd. destruct (HasAmortizedCostSoundnessSoundness_aux os [] Hd) as (d0 & Hd0 & HH).
+  apply has_amortized_cost'.
+  intros os. destruct (physicist's_argument_soundness_aux os [] (bottom_of (exact (eval_trace_from os [])))) as (d0 & Hd0 & HH).
+  { apply bottom_is_least. }
   inversion Hd0; clear Hd0; subst.
-  exact HH.
+  apply (optimistic_mon HH); cbn.
+  intros ? ? [_ INEQ]. fold (cost_trace os) in INEQ.
+  rewrite potential_bottom, Nat.add_0_r in INEQ.
+  exact INEQ.
 Qed.
 
 End Soundness.
@@ -305,7 +387,7 @@ Definition RealTimeCost : Prop :=
 End RealTimeCost.
 
 Definition ImplRealTimeCost
-    (op : Type) (j : CostSpec op) (j' : Cv.Impl op) {IA : ImplApprox j j'}
+    (op : Type) (j : CostSpec op) (j' : Cv.Impl op) {AO : ApproxOrder j j'}
   : Prop :=
   forall (os : list (op * list nat)) (o : op) (ns : list nat),
     ( cost_of (exec_trace (j := j') (os ++ [(o, ns)]) [])
